## <center>数学公式</center>

$a^2+b^2=(a+b)^2-2ab$

a^n+b^n=(a+b)[a^{n-1}-a^{n-2}b^{n-2}+b^{n-1}]\]</p>
    <p><center></center>\[平方差公式:a^2-b^2=(a+b)(a-b)\]</p>
    <p>\[a^n-b^n=(a-b)[a^{n-1}+a^{n-2}b^{n-2}+b^{n-1}]\]</p>
    <p><center>完全平方公式:</center>\[a^2+2ab+b^2=(a+b)^2\]</p>
    <p><center>完全平方公式:</center>\[a^2-2ab+b^2=(a-b)^2\]</p>
    <p><center>立方和公式:</center>\[a^3+b^3=(a+b)(a^2-ab+b^2)\]</p>
    <p><center>立方差公式:</center>\[a^3-b^3=(a-b)(a^2+ab+b^2)\]</p>
    <p><center>完全立方和公式:</center>\[(a+b)^3=a^3+3a^2b+3ab^2+b^3\]</p>
    <p><center>完全立方差公式:</center>\[(a-b)^3=a^3-3a^2b+3ab^2-b^3\]</p>
    <p><center>三项完全平方公式:</center>\[a^2+b^2+c^2=2ab+2bc+2ac=(a+b+c)^2\]</p>
    <p><center>三项立方和公式</center>\[a^3+b^3+c^3-3abc=(a+b+c)(a^2+b^2+c^2-ab-bc-ac)\]</p>

</body>

</html>